spinlock/LockIA.v
@@ -1,156 +1,188 @@
 Require Import CRIS.
-From CRIS.spinlock Require Import Header LockI LockA.
 Require Import ImpPrelude MemA.
 Require Import SchHeader SchA SchTactics.
+From CRIS.spinlock Require Import Header LockI LockA.
 
 Module LockIA. Section LockIA.
   Import LockAS.
   Context `{!crisG Γ Σ α β τ _S _I, !memG, !schG, !spinlockG}.
 
-  Context (E : coPset) (Hsub : ↑N_SpinLockA ⊆ E).
-  Context (tidq : Qp).
-  Context (sp_user : spl_type).
-  Context (sp : sp_type).
-  Context (SchInSp : sp_incl (SchAS.sp sp_user E tidq) sp).
-
+  Context (E : coPset).
+  Context (LockInE: ↑N_SpinLockA ⊆ E).  
+  
   Definition init_cond : iProp Σ := emp%I.
 
   Local Definition MemP := MemP.t.
-  Local Definition SpinLockA := (SpinLockA.t E tidq sp).
-  Local Definition SpinLockI := (SpinLockI.t).
-  Local Definition IstFull := (IstProd (IstSB SpinLockA.(Mod.scopes) IstTrue) IstEq).
-  Local Notation MA := (SpinLockA ★ MemP).
+  Local Definition SpinLockA := SpinLockA.t.
+  Local Definition SpinLockI := SpinLockI.t.
+  Local Definition IstFull := (IstProd (IstSB (Mod.scopes (SpinLockA E)) IstTrue) IstEq).
+  Local Notation MA := (SpinLockA E ★ MemP).
   Local Notation MI := (SpinLockI ★ MemP).
 
-  Lemma newlock_simF : ISim.sim_fun open MA MI init_cond IstFull (Some SpinLockHdr.newlock).
-  Proof using SchInSp Hsub.
+  Lemma newlock_simF :
+    ISim.sim_fun open MA MI init_cond IstFull (Some SpinLockHdr.newlock).
+  Proof.
     init_simF.
+    steps_l; unfold_real_lat_l.
 
-    (* preprocess initial conditions *)
-    steps_l. rename _q1 into tid, _q into vret. destruct _q2 as [n P]; s.
-    iDestruct "ASM" as "[TID [P ->]]". hss.
-    steps_r.
-
-    (* tgt yield *)
-    sch_yield_ir.
+    destruct (arg↓) as [v|] eqn: EQ; cycle 1.
+    { sch_yield_l. steps_l. force_l (tt↑). steps_l.
+      ru_l False%I. iSplitL; cycle 1.
+      { iIntros "F". iExFalso. et. }
+      iIntros ([]) "[_ [[% _] _]]"; subst; hss.
+    }
+    steps_r. sch_yield_rr.
 
     (* tgt inline - mem alloc *)
     steps_r. inline_r. steps_r.
-    unfold_real_lat_r. force_r 1. iSplit; et.
-    iIntros "[%blk [% [PT _]]]".
-    steps_r. hss_r. steps_r.
-
-    (* tgt yield *)
-    sch_yield_ir.
+    unfold_real_lat_r. force_r 1.
+    iSplit; et. iIntros "[%blk [-> [↦ _]]]".
+    steps_r; hss_r; steps_r.
+    sch_yield_rr.
 
     (* tgt inline - mem store *)
     steps_r. inline_r. steps_r.
-    unfold_real_lat_r. force_r (_,_,_,_). s. iFrame. iSplit; et.
-    iIntros "[PT %]".
-    steps_r. hss_r. steps_r.
+    unfold_real_lat_r. force_r (blk, 0%Z, _, _); s.
+    iFrame "↦". iSplit; try done. iIntros "[↦ ->]".
+    steps_r; hss_r; steps_r.
 
     (* src/tgt yield *)
-    sch_yield_ir. steps_r.
-    sch_yield_l. force_l (Vptr (blk, 0%Z)). steps_l. force_l. steps_l.
+    sch_yield_rr. sch_yield_l; steps_l.
 
-    (* prove source postcondition *)
-    (* alloc invariant *)
+    (* lock token allocation *)
     iMod (own_alloc (Excl ())) as "[%γ TKN]"; [done|].
-    iMod (inv_alloc (LockAS.lock_inv (blk, 0%Z) P γ) _ _ _ N_SpinLockA with "[P PT TKN]") as "#I"; eauto.
-    { rewrite /lock_inv /=; SL_red; iRight; iFrame. }
-    forces_l. iFrame. iSplit; eauto.
-    { iSplit; eauto. rewrite /is_lock. iExists _, _; iSplit; eauto. }
-    steps_l. step. eauto.
+    force_l ((Vptr (blk, 0%Z))↑). steps_l.
+    ru_l emp%I.
+    iSplitR "IST"; cycle 1.
+    { iIntros "_". steps_l. sch_yield_l. step. iSplit; done. }
+    iIntros ([n P]) "[W [[_ P] _]]"; s.
+    iSplitR; [eauto|].
+    unfold_pre_post. iRevert "W".
+    iApply (winv_fupd (S n)).
+    iMod (inv_alloc (LockAS.lock_inv (blk, 0%Z) P γ) _ _ _ N_SpinLockA
+      with "[↦ P TKN]") as "#I"; ss.
+    { rewrite /lock_inv; SL_red; iRight; iFrame. }
+    iModIntro; iFrame. iSplit; eauto. iExists _, _; iSplit; eauto.
+    rewrite /is_lock; iExists _; iFrame "I"; done.
+    Unshelve. all: exact 0.
   (*SLOW*)Qed.
 
   Lemma acquire_simF : ISim.sim_fun open MA MI init_cond IstFull (Some SpinLockHdr.acquire).
-  Proof using SchInSp Hsub.
+  Proof.
     init_simF.
+    steps_l; unfold_real_lat_l.
 
-    (* process src precondition *)
-    steps_l. iDestruct "ASM" as "[TID [[-> #LOCK] ->]]". hss.
-    iDestruct "LOCK" as (?) "[% LOCK]". destruct bofs as [blk ofs]. steps_r.
+    (* ill-formed argument *)
+    destruct (arg↓) as [l|] eqn : Heqarg; cycle 1.
+    { sch_yield_l. steps_l. force_l false. force_l (tt↑). steps_l.
+      ru_l False%I. iSplitL; cycle 1.
+      { iIntros "F". iExFalso. et. }
+      iIntros ([[] []]) "[_ [[% _] _]]"; subst; hss.
+    }
+    destruct (or_else (pargs [Tptr] l) (0, 0%Z)) as [blk ofs] eqn: EQ.
+    hss. steps_r.
 
     (* start coinduction for lock acquire/failure *)
-    iApply wsim_reset.
-    iStopProof.
-    revert st_src. combine_quant st_tgt.
+    iApply wsim_reset. iStopProof.
+    revert st_tgt. combine_quant st_src.
     eapply wsim_coind.
-    iIntros (g' _ CIH [st_tgt st_src]) "[#LOCK [IST TID]] /=".
+    iIntros (g' _ CIH [st_src st_tgt]) "IST /=".
     destruct_quant CIH.
 
-    unfold_iterC_r. steps_r.
-    (* tgt yield *)
-    sch_yield_ir.
-    (* open invariant *)
-    iInv "LOCK" as "I" "Hcl". SL_red.
-    iDestruct "I" as "[FAIL|SUCC]".
-    { (* fail case *)
-      (* tgt inline - mem cas *)
-      steps_r. inline_r. steps_r.
-      unfold_real_lat_r. force_r (_,_,_,_,_,_,_,_,_,_). s.
-      iSplitL "FAIL".
-      { iFrame "FAIL"; eauto. }
-      iIntros "[% [PT _]]". steps_r. hss. steps_r.
-      iMod ("Hcl" with "[PT]") as "_". { iFrame. }
-      
-      (* tgt yields *)
-      sch_yield_ir. steps_r.
-      sch_yield_ir. steps_r.
-      by_coind CIH. iFrame. done.
-    }
-    { (* success case *)
-      (* tgt inline - mem cas *)
-      iDestruct "SUCC" as "[POINTS_TO [Q TKN]]".
-      steps_r. inline_r. steps_r.
+    unfold_iter_r. steps_r. sch_yield_rr. sch_yield_l; steps_l.
+    steps_r. inline_r. steps_r.
+    unfold_real_lat_r.
+    ru_r. iIntros (pr) "UPD". rename _q into ret.
 
-      unfold_real_lat_r. force_r (_,_,_,_,_,_,_,_,_,_).
-      iSplitL "POINTS_TO".
-      { iFrame. iSplit; et. }
-      iIntros "[% [PT PRE]]".
-      steps_r. hss_r. steps_r.
-      iMod ("Hcl" with "[PT]") as "_". { iFrame. }
-      (* tgt yields *)
-      do 3 (sch_yield_ir).
-      (* src yield *)
-      sch_yield_l. forces_l. iSplitL "Q TKN TID"; SL_red; iFrame; et.
-      (* both terminate *)
-      step; eauto.
+    destruct (classic (ret = (Vint 0)↑)).
+    { force_l false. steps_l. force_l (Vundef↑). steps_l.
+      ru_l (Own pr)%I.
+      iSplitL "UPD".
+      { iIntros ([[γ vl] [n P]]) "/= [W [[% [%bofs #[% I]]] %]]"; destruct bofs as [blk' ofs'].
+        iRevert "W". iInv "I" as "INV" "ACC". hss.
+        iEval (SL_red) in "INV". iDestruct "INV" as "[PT | [PT [R TKN]]]".
+        { iPoseProof ("UPD" $! (_, _, _, _, _, _, _, _, _, _) with "[PT]") as "> [_ [% _]]".
+          - iFrame "PT". iSplit; eauto.
+          - hss.
+        }
+        iPoseProof ("UPD" $! (_, _, _, _, _, _, _, _, _, _) with "[PT]") as "> [$ [% [↦ _]]] /=".
+        { s. iFrame "PT". iSplit; eauto. }
+        Unshelve. all: try exact 1%Qp; try exact (Vint 0); eauto.
+        hss. iMod ("ACC" with "[↦]") as "_".
+        { SL_red; iFrame "↦". }
+        iIntros "$ !>"; iSplit; et.
+        unfold_pre_post. SL_red. iFrame. et.
+      }
+      iIntros "PR".
+      steps_l. force_r; iFrame. steps_r. hss. steps_r.
+      do 3 sch_yield_rr.
+      sch_yield_l.
+      step. et.
     }
-  Unshelve. all: try exact 1%Qp. all: try exact Vundef.
+    { force_l true. steps_l.
+      ru_l (⌜ret = (Vint 1)↑⌝ ∗ Own pr)%I.
+      iSplitL "UPD".
+      { iIntros ([[γ vl] [n P]]) "/= [W [[% [%bofs #[% I]]] %]]"; destruct bofs as [blk' ofs'].
+        iRevert "W". iInv "I" as "INV" "ACC". hss.
+        iEval (SL_red) in "INV". iDestruct "INV" as "[PT| [PT [R TKN]]]"; cycle 1.
+        { iPoseProof ("UPD" $! (_, _, _, _, _, _, _, _, _, _) with "[PT]") as "> [_ [% _]]".
+          - s. iFrame "PT". iSplit; eauto.
+          - hss.
+        }
+        iPoseProof ("UPD" $! (_, _, _, _, _, _, _, _, _, _) with "[PT]") as "> [$ [% [↦ _]]] /=".
+        { s. iFrame "PT". iSplit; eauto. }
+        Unshelve. all: try exact 1%Qp; try exact (Vint 0); eauto.
+        hss. iMod ("ACC" with "[↦]") as "_".
+        { SL_red; iFrame "↦". }
+        iIntros "$ !>". repeat (iSplit; et).
+        iExists _; iFrame "I"; done.
+      }
+      iIntros "[-> PR]".
+      steps_l. unfold_real_lat_l.
+      force_r; iFrame. steps_r. hss. steps_r.
+      do 2 sch_yield_rr. steps_r.
+      by_coind CIH. iFrame.
+    }
+  Unshelve. all: try exact 1%Qp; try exact (Vint 0); eauto.
   (*SLOW*)Qed.
 
   Lemma release_simF : ISim.sim_fun open MA MI init_cond IstFull (Some SpinLockHdr.release).
-  Proof using SchInSp Hsub.
+  Proof.
     init_simF.
-    (* process src precondition *)
-    steps_l.
-    iDestruct "ASM" as "[TID [(% & #LOCK & TKN & Q) %]]".
-    iDestruct "LOCK" as (?) "[% LOCK]". destruct bofs as [blk ofs].
-    hss.
-    steps_r.
-    (* tgt yield *)
-    sch_yield_ir.
-    (* open invariant *)
-    iInv "LOCK" as "I" "Hcl". SL_red.
-    iDestruct "I" as "[LOCKED|UNLOCKED]".
-    { (* locked case *)
-      steps_r. inline_r. steps_r.
-      unfold_real_lat_r. force_r (_,_,_,_); s.
-      iSplitL "LOCKED"; iFrame; et.
-      iIntros "[PT %]".
-      hss. steps_r. hss_r. steps_r.
-      iMod ("Hcl" with "[PT Q TKN]") as "_".
-      { iRight. iFrame. }
-      (* tgt yield *)
-      sch_yield_ir.
-      (* src yield *)
-      sch_yield_l. steps_l. forces_l. iFrame. iSplit; et. step. iFrame; et.
+    steps_l; unfold_real_lat_l.
+
+    (* ill-formed argument *)
+    destruct (arg↓) as [l|] eqn : Heqarg; cycle 1.
+    { sch_yield_l. steps_l. force_l (tt↑). steps_l.
+      ru_l False%I. iSplitL; cycle 1.
+      { iIntros "F". iExFalso. et. }
+      iIntros ([[] []]) "[_ [[% _] _]]"; subst; hss.
     }
-    { (* unlocked case - ex falso quodlibet *)
-      iDestruct "UNLOCKED" as "[PT [Q' TKN']]".
-      iCombine "TKN TKN'" gives %Hv. done.
+    destruct (or_else (pargs [Tptr] l) (0, 0%Z)) as [blk ofs] eqn: EQ.
+
+    steps_r. sch_yield_rr.
+    steps_r. inline_r. steps_r.
+    unfold_real_lat_r.
+    ru_r. iIntros (pr) "UPD". rename _q into ret.
+    sch_yield_l; steps_l. force_l (Vundef↑). steps_l.
+    ru_l (⌜ret = (Vint 0)↑⌝ ∗ Own pr)%I.
+    iSplitL "UPD".
+    { iIntros ([[γ v] [n R]]) "[W [[% [[% [-> #I]] [TKN R]]] _]] /=". hss.
+      iRevert "W". iInv "I" as "INV" "ACC".
+      iEval (SL_red) in "INV"; iDestruct "INV" as "[PT | [PT [R' TKN']]]"; cycle 1.
+      { SL_red; iCombine "TKN" "TKN'" gives %WF; inv WF. }
+      iPoseProof ("UPD" $! (_, _, _, _) with "[PT]") as "> [$ [↦ %]]".
+      { ss; iFrame "PT"; done. }
+      iMod ("ACC" with "[TKN R ↦]") as "_".
+      { SL_red. iRight; iFrame. }
+      iIntros "$ !>"; eauto.
     }
+
+    iIntros "[-> ?]"; force_r; iFrame.
+    steps_l. steps_r; hss_r. steps_r.
+    sch_yield_rr.
+    sch_yield_l; steps_l; step. et.
+    Unshelve. all: eauto.
   (*SLOW*)Qed.
 
   (* Construct ISim.t for summing up each simulation proofs *)
@@ -166,7 +198,7 @@ Module LockIA. Section LockIA.
   (* ctxr works as a unit in compositions of module simulations *)
   Lemma ctxr :
     ctx_refines
-      (SpinLockA.t E tidq sp ★ MemP.t, emp%I)
-      (SpinLockI.t           ★ MemP.t, emp%I).
+      (SpinLockA.t E ★ MemP.t, emp%I)
+      (SpinLockI.t ★ MemP.t, emp%I).
   Proof. eapply main_adequacy, sim; eauto. Qed.
 End LockIA. End LockIA.
