spinlock/MainIA.v
@@ -13,25 +13,25 @@ Module MainIA. Section MainIA.
   Context `{_spinlockmainG: !spinlockmainG}.
 
   Context (E : coPset) (q: Qp).
-  Context (sp_s sp_t: sp_type). (* sps of lock/sch/mem *)
-  Context (sp_user_s sp_user_t: spl_type).
+  Context (sp_s: sp_type). (* sps of lock/sch/mem *)
+  Context (sp_user_s: spl_type).
+  Context (LockInE: ↑N_SpinLockA ⊆ E).  
   Context (SchInSp_s : sp_incl (SchAS.sp sp_user_s E q) sp_s).
-  Context (SchInSp_t : sp_incl (SchAS.sp sp_user_t E (q / 2)) sp_t).
   Context (MainInSp : spl_sub (MainAS.sp E q) sp_user_s).
 
   Local Definition MemP := MemP.t.
-  Local Definition SpinLockA := (SpinLockA.t E (q / 2) sp_t).
+  Local Definition SpinLockA := SpinLockA.t.
   Local Definition SpinLockMainA := (SpinLockMainA.t E q sp_s).
   Local Definition SpinLockMainI := (SpinLockMainI.t).
   Local Definition IstFull := (IstProd (IstSB SpinLockMainA.(Mod.scopes) IstTrue) IstEq).
-  Local Notation MA := (SpinLockMainA ★ (SpinLockA ★ MemP)).
-  Local Notation MI := (SpinLockMainI ★ (SpinLockA ★ MemP)).
+  Local Notation MA := (SpinLockMainA ★ (SpinLockA E ★ MemP)).
+  Local Notation MI := (SpinLockMainI ★ (SpinLockA E ★ MemP)).
 
   Definition init_cond := MainAS.init_cond E q.
 
   Lemma incr_simF :
     ISim.sim_fun open MA MI init_cond IstFull (Some SpinLockMainHdr.incr).
-  Proof using SchInSp_s SchInSp_t MainInSp.
+  Proof using LockInE SchInSp_s MainInSp.
     init_simF.
     (* process src precondition *)
     steps_l. iDestruct "ASM" as "[TID [[-> [%γ_l [#I F]]] ->]]". hss.
@@ -40,62 +40,65 @@ Module MainIA. Section MainIA.
     (* main code *)
     steps_l. hss. steps_l. rewrite /SpinLockMainA.incr. steps_l.
     steps_r. hss. steps_r. rewrite /SpinLockMainI.incr. steps_r.
-    (* tgt yields *)
-    sch_yield_ir.
-    steps_r.
-    (* tgt inline - lock acquire *)
-    sch_yield_ir.
-    steps_r. inline_r. force_r (tid, (γ_l, Vptr (blk_l, ofs_l), existT 0 (lock_P (blk_v, ofs_v) γ_v))).
-    steps_r. forces_r.
-    rewrite -{1}(Qp.div_2 q); iPoseProof (SchAS.tid_user_split with "TID") as "[TID1 ITD2]".
-    iFrame. iSplit; eauto. hss. steps_r.
-    sch_yield_ii; [erewrite Qp.div_2; et|].
+    sch_yield_ir. steps_r.
 
-    (* (* success case *) *)
-    steps_r. iDestruct "GRT" as "[TID' [[-> [TKN P]] _]]". hss. steps_r.
-    iPoseProof (SchAS.tid_user_merge with "[TID TID']") as "TID"; iFrame; rewrite Qp.div_2.
-    (* tgt yield *)
-    sch_yield_ir.
-    rewrite /lock_P; SL_red; iDestruct "P" as "[%x P]"; SL_red; iDestruct "P" as "[PT P]".
+    (* tgt inline - lock acquire *)
+    sch_yield_ir. steps_r.
+    inline_r. steps_r.
+    real_lat_ir "IST TID".
+    { iFrame. instantiate (1:= (_,_,existT _ _)); s.
+      iModIntro. iSplit; et.
+      iIntros "[W [[% _] %]]". hss.
+    }
+    steps_r. ru_r. iIntros (?) "SIM". unfold_pre_post.
+    iApply wsim_unfold; iIntros "W".
+    iMod ("SIM" $! (_,_,existT _ _) with "[W]") as "[PR [W2 [[-> [TKN P]] _]]]".
+    { iFrame "I". iFrame. et. }
+    SL_red; iDestruct "P" as "[%x P]"; SL_red; iDestruct "P" as "[PT P]".
+    iApply wsim_fold; iFrame.
+    forces_r; iFrame.
+    steps_r. sch_yield_ir. steps_r. hss. steps_r. sch_yield_ir.
+
     (* tgt inline - mem load *)
-    steps_r. inline_r. steps_r.
-    unfold_real_lat_r. force_r (blk_v, ofs_v, 1%Qp, Vint x).
-    iSplitL "PT"; iFrame; eauto.
-    iIntros "[PT %]". hss. steps_r. hss_r; steps_r.
-    (* tgt yield *)
-    do 2 (sch_yield_ir).
-    (* tgt inline - mem store *)
-    steps_r. inline_r. steps_r.
-    unfold_real_lat_r. force_r (blk_v, ofs_v, _, Vint (x + 1)).
+    steps_r. inline_r. steps_r. unfold_real_lat_r.
+    force_r (blk_v, ofs_v, 1%Qp, Vint x).
     iSplitL "PT"; iFrame; et.
-    iIntros "[PT %]". steps_r. hss_r; steps_r.
-    sch_yield_ir.
+    iIntros "[PT ->]". steps_r. hss. steps_r.
+    sch_yield_ir. steps_r. sch_yield_ir. steps_r.
+
+    (* tgt inline - mem store *)
+    steps_r. inline_r. steps_r. unfold_real_lat_r.
+    force_r (blk_v, ofs_v, _, Vint (x + 1)).
+    iSplitL "PT"; iFrame; et.
+    iIntros "[PT ->]". steps_r. hss. steps_r.
+    sch_yield_ir. steps_r.
+
     iCombine "P F" as "C". iMod (own_update with "C") as "[F C]".
     { apply frac_auth_update, (Z_local_update _ _ (x + 1) 1); lia. }
+
     (* tgt inline - lock acquire - restore lock protected proposition *)
-    steps_r. inline_r. steps_r. force_r (tid, (γ_l, Vptr (blk_l, ofs_l), existT 0 (lock_P (blk_v, ofs_v) γ_v))).
-    rewrite -{1}(Qp.div_2 q); iPoseProof (SchAS.tid_user_split with "TID") as "[TID1 ITD2]".
-    forces_r. iSplitL "TID1 F PT TKN".
+    steps_r. inline_r. steps_r. unfold_real_lat_r.
+    sch_yield_ir. steps_r.
+    iApply wsim_unfold; iIntros "W".
+    force_r (γ_l, Vptr (blk_l, ofs_l), existT 0 (lock_P (blk_v, ofs_v) γ_v)).
+    iSplitL "W F PT TKN".
     { SL_red. rewrite /lock_P; ss.
-      iFrame "TID1". iSplit; iFrame; eauto. iSplit; eauto. iSplit.
-      { iExact "I". }
-      { iExists _; SL_red; iFrame. }
+      iFrame "I". iFrame. repeat (iSplit; et). 
+      iExists _; SL_red; iFrame.
     }
-    steps_r. hss. steps_r.
-    (* tgt yield *)
-    sch_yield_ii; [erewrite Qp.div_2; et|].
-    steps_r. iDestruct "GRT" as "[TID' [-> _]]". hss. steps_r.
-    iPoseProof (SchAS.tid_user_merge with "[TID TID']") as "TID"; iFrame; rewrite Qp.div_2.
-    sch_yield_ir.
-    (* src yield *)
-    sch_yield_l. steps_l. forces_l. iFrame; iSplit; eauto.
-    (* both terminate *)
-    step. iFrame. eauto.
+    s. iIntros "[W %]"; des; subst.
+    iApply wsim_fold; iFrame.
+    
+    steps_r. sch_yield_ir. steps_r. hss. steps_r. sch_yield_ir. steps_r.
+    sch_yield_l. steps_l.
+    iApply wsim_unfold; iIntros "W".
+    forces_l. iFrame. iSplit; et.
+    step. et.
   (*SLOW*)Qed.
 
   Lemma main_simF :
     ISim.sim_fun open MA MI init_cond IstFull None.
-  Proof using SchInSp_s SchInSp_t MainInSp.
+  Proof using LockInE SchInSp_s MainInSp.
     init_simF.
     rewrite /Sch.spawn /Sch.join.
 
@@ -104,42 +107,38 @@ Module MainIA. Section MainIA.
     iAssert (IstFull [] []) as "IST".
     { do 4 (iExists []). iPureIntro. esplits; et; ss. }
     iRevert "IST"; iIntros "IST"; rewrite bi.intuitionistically_elim.
-
-    steps_l. steps_r.
-    (* tgt yield *)
-    sch_yield_ir.
+    steps_l. steps_r. sch_yield_ir.
 
     (* tgt inline - mem alloc - counter allocation *)
-    steps_r. inline_r. steps_r.
-    unfold_real_lat_r. force_r 1; iSplit; eauto.
-    iIntros "[%blk [% [GRT _]]]"; hss. steps_r. hss_r; steps_r.
-    sch_yield_ir.
+    steps_r. inline_r. steps_r. unfold_real_lat_r.
+    force_r 1. iSplit; eauto.
+    iIntros "[%blk [-> [GRT _]]]". steps_r. hss. steps_r. sch_yield_ir.
+
     (* tgt inline - mem store - counter initialization *)
-    steps_r. inline_r. steps_r.
-    unfold_real_lat_r. force_r (blk, 0%Z, _, Vint 0).
+    steps_r. inline_r. steps_r. unfold_real_lat_r.
+    force_r (blk, 0%Z, _, Vint 0). s.
     iFrame; iSplit; eauto.
-    iIntros "[PT %]". steps_r. hss. steps_r.
-    sch_yield_ir.
+    iIntros "[PT ->]". steps_r. hss. steps_r. sch_yield_ir.
+
     (* create lock-guarded proposition *)
     iApply (wsim_own_alloc (●F 0%Z ⋅ ◯F{1} 0%Z)).
     { eapply frac_auth_valid; ss. }
     iIntros "[%γ [B W]]".
+
     (* tgt inline - newlock *)
-    steps_r. inline_r. steps_r.
-    force_r (0, existT 0 (lock_P (blk, 0%Z) γ)). forces_r.
-    rewrite -{1}(Qp.div_2 q); iPoseProof (SchAS.tid_user_split with "TID") as "[TID1 ITD2]".
-    iSplitL "TID1 B PT"; eauto.
-    { iFrame; SL_red; iSplit; eauto. iFrame. iExists _; SL_red; iFrame. }
-    steps_r. hss. steps_r.
-    (* src/tgt yields *)
-    sch_yield_ii; [erewrite Qp.div_2; et|].
-    steps_r. iDestruct "GRT" as "[TID' [[%val [%γ_l [-> #I]]] %EQ]]".
-    hss. steps_r.
-    iPoseProof (SchAS.tid_user_merge with "[TID TID']") as "TID"; iFrame; rewrite Qp.div_2.
-    sch_yield_ir.
-    iPoseProof "I" as "[%bofs_l [-> _]]".
-    sch_yield_l. steps_l. force_l (Vptr bofs_l, Vptr (blk, 0%Z)). steps_l. sch_yield_l.
-    (* create preconditions of incr *)
+    steps_r. inline_r. steps_r. unfold_real_lat_r. sch_yield_ir. steps_r.
+    iApply wsim_unfold. iIntros "I".
+    force_r (existT 0 (lock_P (blk, 0%Z) γ)).
+    iSplitL "B I PT"; eauto.
+    { iFrame. s. SL_red; iSplit; eauto. iSplit; et.
+      iFrame. iExists _; SL_red; iFrame. }
+    iIntros "[WINV [[%v [%γ_l [-> #I]]] %EQ]]". hss.
+    iApply wsim_fold; iFrame.
+    steps_r. sch_yield_ir. steps_r. hss. steps_r. sch_yield_ir.
+    sch_yield_l. steps_l. force_l (v, Vptr (blk, 0%Z)).
+    steps_l. sch_yield_l.
+
+    iPoseProof "I" as "[%bofs [-> _]]".
     iDestruct "W" as "[W1 W2]".
 
     (* spawn thread 1 - incr *)
@@ -150,8 +149,7 @@ Module MainIA. Section MainIA.
     }
     call "IST".
     steps_l. iDestruct "ASM" as "[% [-> [TID [% [[-> ->] TKN1]]]]]".
-    rename _q0 into tid1.
-    steps_r. hss. steps_r.
+    rename _q0 into tid1. steps_r. hss. steps_r.
     sch_yield_ir. sch_yield_l.
 
     (* spawn thread 2 - incr *)
@@ -161,9 +159,8 @@ Module MainIA. Section MainIA.
       - iFrame; et.
     }
     call "IST".
-    steps_l. iDestruct "ASM" as "[% [-> [TID [% [[-> ->] TKN2]]]]]". hss.
-    rename _q0 into tid2.
-    steps_r. hss. steps_r.
+    steps_l. iDestruct "ASM" as "[% [-> [TID [% [[-> ->] TKN2]]]]]".
+    rename _q0 into tid2. steps_r. hss. steps_r.
     sch_yield_ir. sch_yield_l.
 
     (* join thread 1 - incr *)
@@ -171,8 +168,7 @@ Module MainIA. Section MainIA.
     { iExists _. do 2 (iSplit; et). iFrame. }
     call "IST".
     steps_l. iDestruct "ASM" as "[% [-> [% [% [[-> ->] [TID W1]]]]]]".
-    hss. rename _q1 into vret.
-    steps_r. hss. steps_r.
+    rename _q1 into vret1. steps_r. hss. steps_r.
     sch_yield_ir. sch_yield_l.
 
     (* join thread 2 - incr *)
@@ -180,51 +176,48 @@ Module MainIA. Section MainIA.
     { iExists _. do 2 (iSplit; et). iFrame. }
     call "IST".
     steps_l. iDestruct "ASM" as "[% [-> [% [% [[-> ->] [TID W2]]]]]]".
-    hss. rename _q1 into vret0.
-    steps_r. hss. steps_r.
+    rename _q1 into vret2. steps_r. hss. steps_r.
     sch_yield_ir.
 
     (* tgt inline - lock acquire *)
     steps_r. inline_r. steps_r.
-    force_r (_, (γ_l, Vptr bofs_l, existT 0 (lock_P (blk, 0%Z) γ))). forces_r.
-    rewrite -{1}(Qp.div_2 q); iPoseProof (SchAS.tid_user_split with "TID") as "[TID1 ITD2]".
+    real_lat_ir "IST TID".
+    { instantiate (1:= (_,_,existT _ _)). s.
+      iFrame. iModIntro. iSplit; et.
+      iIntros "[W _]"; et.
+    }
+    iApply wsim_unfold; iIntros "WINV".
+    steps_r. force_r (γ_l, Vptr bofs, existT 0 (lock_P (blk, 0%Z) γ)). s.
     iFrame. iSplit; eauto.
-    steps_r. hss. steps_r.
-    sch_yield_ii; [erewrite Qp.div_2; et|].
-    steps_r. iDestruct "GRT" as "[TID' [[-> [TKN P]] _]]". hss. steps_r.
+    iIntros "[WINV [[% [TKN P]] _]]"; hss.
     SL_red. iCombine "W1 W2" as "W".
     iDestruct "P" as "[%x P]"; SL_red; iDestruct "P" as "[PT B]".
     iCombine "B W" gives %WF%frac_auth_agree. inv WF.
-    iPoseProof (SchAS.tid_user_merge with "[TID TID']") as "TID"; iFrame; rewrite Qp.div_2.
-    sch_yield_ir.
+    iApply wsim_fold; iFrame.
+    steps_r. sch_yield_ir. steps_r. hss. steps_r. sch_yield_ir.
+    
     (* tgt inline - mem load *)
-    steps_r. inline_r. steps_r.
-    unfold_real_lat_r. force_r (blk, 0%Z, 1%Qp, Vint 2%Z); s.
-    iFrame "PT". iSplit; et.
-    iIntros "[PT %]". steps_r. hss. steps_r.
-    (* tgt yield *)
-    do 2 (sch_yield_ir).
+    steps_r. inline_r. steps_r. unfold_real_lat_r.
+    force_r (blk, 0%Z, 1%Qp, Vint 2%Z); s.
+    iSplitL "PT"; eauto. iIntros "[PT ->]".
+    steps_r. hss. steps_r. sch_yield_ir. steps_r. sch_yield_ir.
+    
     (* tgt inline - lock release *)
     steps_r. inline_r. steps_r.
-    force_r (_, (γ_l, Vptr bofs_l, existT 0 (lock_P (blk, 0%Z) γ))). forces_r.
-    rewrite -{1}(Qp.div_2 q); iPoseProof (SchAS.tid_user_split with "TID") as "[TID1 ITD2]".
-    iSplitL "TKN TID1 B PT".
-    { iFrame; SL_red. iSplit; eauto. iFrame. iSplit; eauto. iSplit; eauto.
-      iExists _; SL_red; iFrame.
-    }
-    steps_r. hss. steps_r.
-    (* tgt yield *)
-    sch_yield_ii; [erewrite Qp.div_2; et|].
-    steps_r. iDestruct "GRT" as "[TID' [-> _]]". hss. steps_r.
-    iPoseProof (SchAS.tid_user_merge with "[TID TID']") as "TID"; iFrame; rewrite Qp.div_2.
-    sch_yield_ir.
+    unfold_real_lat_r. sch_yield_ir. steps_r.
+    iApply wsim_unfold; iIntros "WINV".
+    force_r (γ_l, Vptr bofs, existT 0 (lock_P (blk, 0%Z) γ)). s.
+    iSplitL "WINV TKN B PT".
+    { iFrame; SL_red. repeat (iSplit; et; iFrame). iExists _; SL_red; iFrame. }
+    iIntros "[WINV [-> _]]".
+    iApply wsim_fold; iFrame.
+    steps_r. sch_yield_ir. steps_r. hss. steps_r. sch_yield_ir.
+
     (* both output - counter value *)
-    sch_yield_l. step.
-    steps_l. steps_r.
-    sch_yield_ir.
-    sch_yield_l. 
+    sch_yield_l. step. steps_l. steps_r. sch_yield_ir. sch_yield_l.
+
     (* terminate both *)
-    step. iSplit; eauto.
+    step. et.
   (*SLOW*)Qed.
 
   Lemma sim : ISim.t open MA MI init_cond IstFull.
@@ -235,8 +228,8 @@ Module MainIA. Section MainIA.
   Qed.
 
   Definition ctxr :
-    ctx_refines
-    ((SpinLockMainA.t E q sp_s) ★ ((SpinLockA.t E (q/2) sp_t) ★ MemP.t), init_cond)
-    ((SpinLockMainI.t)          ★ ((SpinLockA.t E (q/2) sp_t) ★ MemP.t), emp%I).
+  ctx_refines
+  ((SpinLockMainA.t E q sp_s) ★ ((SpinLockA.t E) ★ MemP.t), init_cond)
+  ((SpinLockMainI.t)          ★ ((SpinLockA.t E) ★ MemP.t), emp%I).
   Proof. eapply main_adequacy, sim. Qed.
 End MainIA. End MainIA.
