incr_faa/FaaI.v
@@ -1,6 +1,6 @@
 Require Import CRIS.
 Require Import ImpPrelude MemHeader MemA SchA SchTactics SchHeader.
-From CRIS.incr Require Import Header.
+From CRIS.incr_faa Require Import Header.
 
 Module FaaI. Section FaaI.
   Context {Σ : GRA}.
