spinlock_na/LockI.v
@@ -1,5 +1,5 @@
 Require Import CRIS.
-From CRIS.spinlock_atomic Require Import Header.
+From CRIS.spinlock_na Require Import Header.
 Require Import ImpPrelude SchHeader MemHeader.
 
 (* Implementation of the spinlock library *)
@@ -21,7 +21,7 @@ Module SpinLockI. Section SpinLockI.
 
   Definition acquire : list val → itree crisE val :=
     λ x,
-      (ITree.iter
+      (iterC
         (λ _,
           𝒴;;; 'b_raw : val <- ccallU MemHdr.cas (x ++ [Vint 0; Vint 1]);;
           𝒴;;; 'b : Z <- (pargs [Tint] [b_raw])?;;
